Clean up interface

ctx-equiv-ixfree/interface.v
@@ -1,124 +1,80 @@
 
-From Stdlib Require Import Utf8.
-From Binding Require Import Lib Auto.
-Require Import Binding.Set.
-
-From Stdlib Require Import Classes.Morphisms Program.
+From Stdlib Require Import Utf8 Classes.Morphisms Program.
 
 Module Type StagedLogic.
 
+  (* Binding *)
+  Parameter inc : Set → Set.
+  Parameter empty : Set.
+  Notation "∅" := empty.
+  Parameter v : ∀ {V}, nat → V.
+  Notation "& n" := (v n) (at level 5).
+
+  (* Expressions *)
   Parameter expr : Set → Set.
-  Parameter val : Set → Set.
-
-  Parameter ret : ∀ {V:Set}, val V → expr V.
   Parameter app : ∀ {V:Set}, expr V → expr V → expr V.
-  Parameter var : ∀ {V:Set}, V → val V.
-  Parameter lambda : ∀ {V:Set}, expr (inc V) → val V.
+  Parameter var : ∀ {V:Set}, V → expr V.
+  Parameter lambda : ∀ {V:Set}, expr (inc V) → expr V.
 
-  Parameter emap : ∀ {A B:Set}, (A [→] B) → expr A → expr B.
-  Parameter vmap : ∀ {A B:Set}, (A [→] B) → val A → val B.
-
-  (* equivalence *)
+  (* Equivalence *)
   Parameter eqv : ∀ {V}, expr V → expr V → Prop.
   Parameter Reflexive_eqv : ∀ {V:Set}, Reflexive (@eqv V).
   Parameter Symmetric_eqv : ∀ {V:Set}, Symmetric (@eqv V).
   Parameter Transitive_eqv : ∀ {V:Set}, Transitive (@eqv V).
 
-  (* entailment *)
+  (* Entailment *)
   Parameter entails : ∀ {V}, expr V → expr V → Prop.
   Parameter Reflexive_entails : ∀ {V:Set}, Reflexive (@entails V).
   Parameter Transitive_entails : ∀ {V:Set}, Transitive (@entails V).
 
-(* TODO just have one expr type? *)
-
-  (* equivalence for values *)
-  Parameter eqv_val : ∀ {V}, val V → val V → Prop.
-  Parameter Reflexive_eqv_val : ∀ {V:Set}, Reflexive (@eqv_val V).
-  Parameter Symmetric_eqv_val : ∀ {V:Set}, Symmetric (@eqv_val V).
-  Parameter Transitive_eqv_val : ∀ {V:Set}, Transitive (@eqv_val V).
-
-  Parameter Proper_eqv_app : ∀ {V:Set}, Proper (@eqv V ==> @eqv V ==> @eqv V) app.
+  (* Proper instances *)
   Parameter Proper_iff_eqv : ∀ {V:Set}, Proper (@eqv V ==> @eqv V ==> iff) eqv.
-  Parameter Proper_eqv_lambda : ∀ {V:Set}, Proper (@eqv (inc V) ==> @eqv_val V) lambda.
+  Parameter Proper_eqv_app : ∀ {V:Set}, Proper (@eqv V ==> @eqv V ==> @eqv V) app.
+  Parameter Proper_eqv_lambda : ∀ {V:Set}, Proper (@eqv (inc V) ==> @eqv V) lambda.
 
   Parameter Proper_impl_entails : ∀ {V:Set},
     Proper (flip (@entails V) ==> @entails V ==> impl) entails.
   Parameter Proper_entails_app : ∀ {V:Set},
     Proper (@entails V ==> @entails V ==> @entails V) app.
+  Parameter Proper_entails_lambda : ∀ {V:Set},
+    Proper (@entails (inc V) ==> @entails V) lambda.
 
-  Section Bind.
+  (* Substitution *)
+  Parameter subst : ∀ {V}, expr (inc V) → expr V → expr V.
+  (* TODO equations *)
 
-  Context `{SetPureCore val}.
-
-  Parameter ebind : ∀ {A B:Set}, (A [⇒] B) → expr A → expr B.
-  Parameter vbind : ∀ {A B:Set}, (A [⇒] B) → val A → val B.
-
-  Context `{BindCore Set (@Sub val _) expr}.
-
-  Parameter red_beta : ∀ {V} (e:expr (inc V)) (v:val V),
-    eqv
-      (app (ret (lambda e)) (ret v))
-      (subst e v).
-
-  End Bind.
+  (* Lemmas *)
+  Parameter red_beta : ∀ {V} (e:expr (inc V)) (v:expr V),
+    eqv (app (lambda e) v) (subst e v).
 
 End StagedLogic.
 
-Module MakeInstances (SL: StagedLogic).
+Module WithInstances (SL: StagedLogic).
 
   Import SL.
 
   #[global]
-  Instance SetPureCore_value : SetPureCore val :=
-    { set_pure := @var }.
+  Instance Reflexive_eqv {V:Set} : Reflexive (@eqv V) := Reflexive_eqv.
 
   #[global]
-  Instance FunctorCore_emap : FunctorCore expr := @emap.
+  Instance Proper_eqv_app {V:Set} : Proper (@eqv V ==> @eqv V ==> @eqv V) app :=
+    Proper_eqv_app.
 
   #[global]
-  Instance FunctorCore_vmap : FunctorCore val := @vmap.
+  Instance Proper_iff_eqv {V:Set} : Proper (@eqv V ==> @eqv V ==> iff) eqv :=
+    Proper_iff_eqv.
 
   #[global]
-  Instance BindCore_ebind : BindCore expr := @ebind SetPureCore_value.
-
-  #[global]
-  Instance BindCore_vbind : BindCore val := @vbind SetPureCore_value.
-
-  #[global]
-  Instance Reflexive_eqv : ∀ {V:Set}, Reflexive (@eqv V).
-  Proof.
-    intros.
-    eapply Reflexive_eqv.
-  Qed.
-
-  #[global]
-  Instance Proper_eqv_app : ∀ {V:Set}, Proper (@eqv V ==> @eqv V ==> @eqv V) app.
-  Proof.
-    intros.
-    eapply Proper_eqv_app.
-  Qed.
-
-  #[global]
-  Instance Proper_iff_eqv : ∀ {V:Set}, Proper (@eqv V ==> @eqv V ==> iff) eqv.
-  Proof.
-    intros.
-    eapply Proper_iff_eqv.
-  Qed.
-
-  #[global]
-  Instance Proper_eqv_lambda : ∀ {V:Set}, Proper (@eqv (inc V) ==> @eqv_val V) lambda.
-  Proof.
-    intros.
-    eapply Proper_eqv_lambda.
-  Qed.
+  Instance Proper_eqv_lambda {V:Set} : Proper (@eqv (inc V) ==> @eqv V) lambda :=
+    SL.Proper_eqv_lambda.
 
   Export SL.
 
-End MakeInstances.
+End WithInstances.
 
 Module CaseStudy (SL : StagedLogic).
 
-  Module M := MakeInstances(SL).
+  Module M := WithInstances(SL).
   Import M.
 
   Parameter red_hello : ∀ {V} (e1 e2:expr V), eqv e1 e2.
@@ -130,16 +86,15 @@ Module CaseStudy (SL : StagedLogic).
     reflexivity.
   Qed.
 
-  Definition id_exp : expr ∅ := ret (lambda (ret (var &0))).
+  Definition id_exp : expr ∅ := lambda (var &0).
 
-  Example e2 (v1:val ∅) (e2:expr ∅):
-    eqv (app (app id_exp (ret v1)) e2) (app (ret v1) e2).
+  Example e2 (e1 e2:expr ∅):
+    eqv (app (app id_exp e1) e2) (app (e1) e2).
   Proof.
     unfold id_exp.
     (* rewrite (red_beta (ret (var &0)) v1). *)
     rewrite red_beta.
-    simpl.
-    (* cannot perform this subst without a definition for bind *)
+    (* need equations for subst *)
   Abort.
 
 End CaseStudy.
